

Left Recursion

Lecture 6

Section 4.3.3

ROKAN UDDIN FARUQUI

Associate Professor
Dept of Computer Science and Engineering
University of Chittagong, Bangladesh
Email: *rokan@cu.ac.bd*

- 1 Problems with Recursive Descent
- 2 Left Recursion
- 3 Eliminating Left Recursion
- 4 Advantages of Left Recursion
- 5 Assignment



Outline

- 1 Problems with Recursive Descent
- 2 Left Recursion
- 3 Eliminating Left Recursion
- 4 Advantages of Left Recursion
- 5 Assignment



A Problem with Recursive Descent Parsers

- Suppose the grammar were

$$S \rightarrow AB \mid CD$$

$$A \rightarrow BC \mid CA \mid a$$

$$B \rightarrow CA \mid DB \mid b$$

$$C \rightarrow BA \mid AD \mid a$$

$$D \rightarrow AC \mid BD \mid b$$

- How could a top-down parser decide which production for S to use to derive **babbb**?
- Indeed, can **babbb** be derived?



A Problem with Recursive Descent Parsers

- Suppose the grammar were

$$S \rightarrow AB \mid CD$$

$$A \rightarrow BC \mid CA \mid \mathbf{a}$$

$$B \rightarrow CA \mid DB \mid \mathbf{b}$$

$$C \rightarrow BA \mid AD \mid \mathbf{a}$$

$$D \rightarrow AC \mid BD \mid \mathbf{b}$$

- How could a top-down parser decide which production for S to use to derive **babbb**?
- Indeed, can **babbb** be derived?



Another Problem with Recursive Descent Parsers

```
SO {
  SO;
  SO;
}
```

- Suppose the grammar were

$$S \rightarrow S S \mid a$$

- How could the parser decide how many times to use the production $S \rightarrow S S$ before using the production $S \rightarrow a$?



Futile Attempt

Futile Attempt

```
void S()      // Match S -> S S | a
{
    if (token == a)
        match(a);
    else
    {
        S();
        S();
    }
    return;
}
```



Outline

- 1 Problems with Recursive Descent
- 2 Left Recursion**
- 3 Eliminating Left Recursion
- 4 Advantages of Left Recursion
- 5 Assignment



Left Recursion

Definition (Left recursive production)

A production is **left recursive** if it is of the form

$$A \rightarrow A\alpha.$$

for some nonterminal A and some string α .

Definition (Left recursive grammar)

A grammar is **left recursive** if there is a derivation

$$A \xRightarrow{+} A\alpha$$

for some nonterminal A and some string α .

Left Recursion

Left Recursion

```
void A()          // Match  $A \rightarrow A$ 

{
    A();
    // Process

    return;
}
```

- Attempting to match the left-recursive production $A \rightarrow A\alpha$.



Left Recursion

$$S \rightarrow AB \mid CD$$

$$A \rightarrow BC \mid CA \mid \mathbf{a}$$

$$B \rightarrow CA \mid DB \mid \mathbf{b}$$

$$C \rightarrow BA \mid AD \mid \mathbf{a}$$

$$D \rightarrow AC \mid BD \mid \mathbf{b}$$

- Is this grammar left recursive?



Left Recursion

- Recall that in the earlier example, we added the production

$$S' \rightarrow SS' \mid \varepsilon,$$

not the production

$$S' \rightarrow S'S \mid \varepsilon.$$

- Why?
- Are they equivalent as far as the language of the grammar is concerned?



Outline

- 1 Problems with Recursive Descent
- 2 Left Recursion
- 3 Eliminating Left Recursion**
- 4 Advantages of Left Recursion
- 5 Assignment



Eliminating Left Recursion

- Left recursion in a production may be removed by transforming the grammar in the following way.
- Replace

$$A \rightarrow A\alpha \mid \beta$$

with

$$\begin{aligned} A &\rightarrow \beta A' \\ A' &\rightarrow \alpha A' \mid \epsilon. \end{aligned}$$

where A' is a new nonterminal.



Eliminating Left Recursion

- Under the original productions, a derivation of $\beta\alpha\alpha\alpha$ is

$$\begin{aligned} A &\Rightarrow A\alpha \\ &\Rightarrow A\alpha\alpha \\ &\Rightarrow A\alpha\alpha\alpha \\ &\Rightarrow \beta\alpha\alpha\alpha. \end{aligned}$$



Eliminating Left Recursion

- Under the new productions, a derivation of $\beta\alpha\alpha\alpha$ is

$$\begin{aligned} A &\Rightarrow \beta A' \\ &\Rightarrow \beta\alpha A' \\ &\Rightarrow \beta\alpha\alpha A' \\ &\Rightarrow \beta\alpha\alpha\alpha A' \\ &\Rightarrow \beta\alpha\alpha\alpha. \end{aligned}$$



Example

Example (Eliminating Left Recursion)

- Consider the left recursive grammar

$$E \rightarrow E + T \mid T$$

$$T \rightarrow T * F \mid F$$

$$F \rightarrow (E) \mid \text{id}$$



Example

Example (Eliminating Left Recursion)

- Apply the transformation to E :

$$\begin{aligned}E &\rightarrow T E' \\ E' &\rightarrow + T E' \mid \varepsilon.\end{aligned}$$

- Then apply the transformation to T :

$$\begin{aligned}T &\rightarrow F T' \\ T' &\rightarrow * F T' \mid \varepsilon.\end{aligned}$$

Example

Example (Eliminating Left Recursion)

- Apply the transformation to E :

$$\begin{aligned}E &\rightarrow T E' \\ E' &\rightarrow + T E' \mid \varepsilon.\end{aligned}$$

- Then apply the transformation to T :

$$\begin{aligned}T &\rightarrow F T' \\ T' &\rightarrow * F T' \mid \varepsilon.\end{aligned}$$

Example

Example (Eliminating Left Recursion)

- Now the grammar is

$$E \rightarrow T E'$$

$$E' \rightarrow + T E' \mid \varepsilon$$

$$T \rightarrow F T'$$

$$T' \rightarrow * F T' \mid \varepsilon$$

$$F \rightarrow (E) \mid \text{id}$$



Eliminating Left Recursion

Eliminating Left Recursion

```
void Eprime()      // Match  $E' \rightarrow + T E'$ 
{
    if (token == PLUS)
    {
        match(PLUS);
        T();
        Eprime();
    }
    return;
}
```

- This is the function for E' .



Outline

- 1 Problems with Recursive Descent
- 2 Left Recursion
- 3 Eliminating Left Recursion
- 4 Advantages of Left Recursion
- 5 Assignment

Advantages of Left Recursion

- A left recursive grammar is often more intuitive than the transformed grammar.
- A left recursive grammar will match expressions earlier, leading to shallower recursion.
- Bottom-up parsing takes advantage of the benefits of left recursion.



Example

- Consider the simple grammar

$$E \rightarrow E + E \mid \text{id}$$

- Convert it to

$$\begin{aligned} E &\rightarrow \text{id } E' \\ E' &\rightarrow + E E' \mid \varepsilon \end{aligned}$$



Outline

- 1 Problems with Recursive Descent
- 2 Left Recursion
- 3 Eliminating Left Recursion
- 4 Advantages of Left Recursion
- 5 Assignment**



Assignment

Homework

- 4.2.1, 4.2.2.
- 4.4.1, 4.4.3, 4.4.4
- The grammar

$$R \rightarrow R \cup R \mid R R \mid R^* \mid (R) \mid \mathbf{a} \mid \mathbf{b}$$

generates all regular expressions over the alphabet $\{\mathbf{a}, \mathbf{b}\}$.

- Rewrite the grammar to reflect the precedence rules.
- Eliminate left recursion.

